compiler/backend/passes/proofs/state_namesProofScript.sml
@@ -189,54 +189,54 @@ Proof
   \\ drule compile_rel_itree_of \\ fs []
 QED
 
-Theorem give_names_cexp_wf:
+Theorem give_names_cexp_wwf:
     ∀x e n.
     give_names x = (e,n) ⇒
-    cexp_wf x ⇒ cexp_wf e
+    cexp_wwf x ⇒ cexp_wf e
 Proof
   ho_match_mp_tac give_names_ind \\ rpt strip_tac
   >~[‘Var’]
-  >- (fs [give_names_def, cexp_wf_def]
+  >- (fs [give_names_def, cexp_wwf_def]
       \\ rw [cexp_wf_def])
   >~[‘Lam vn’]
-  >- (fs [give_names_def, cexp_wf_def]
-      \\ Cases_on ‘vn’ \\ fs [cexp_wf_def]
-      \\ pairarg_tac \\ fs [cexp_wf_def]
+  >- (fs [give_names_def, cexp_wwf_def]
+      \\ pairarg_tac \\ fs []
+      \\ Cases_on ‘vn’ \\ fs []
       \\ rw [cexp_wf_def])
   >~[‘Let vn’]
-  >- (fs [give_names_def, cexp_wf_def]
+  >- (fs [give_names_def, cexp_wwf_def]
       \\ Cases_on ‘vn’ \\ fs [cexp_wf_def]
       \\ pairarg_tac \\ fs [cexp_wf_def]
       \\ pairarg_tac \\ fs [cexp_wf_def]
       \\ rw [cexp_wf_def])
   >~[‘App’]
-  >- (fs [give_names_def, cexp_wf_def]
+  >- (fs [give_names_def, cexp_wwf_def]
       \\ rw [cexp_wf_def, EVERY_MEM, MEM_MAP]
       \\ last_x_assum $ drule_then assume_tac
       \\ rename1 ‘give_names a’
       \\ Cases_on ‘give_names a’ \\ fs [EVERY_MEM])
   >~[‘Handle’]
-  >- (fs [give_names_def, cexp_wf_def]
+  >- (fs [give_names_def, cexp_wwf_def]
       \\ pairarg_tac \\ fs []
       \\ pairarg_tac \\ fs []
       \\ rw [cexp_wf_def])
   >~[‘HandleApp’]
-  >- (fs [give_names_def, cexp_wf_def]
+  >- (fs [give_names_def, cexp_wwf_def]
       \\ pairarg_tac \\ fs []
       \\ pairarg_tac \\ fs []
-      \\ rw [cexp_wf_def])
+      \\ rw [cexp_wf_def, op_args_ok_def])
   >~[‘If’]
-  >- (fs [give_names_def, cexp_wf_def]
+  >- (fs [give_names_def, cexp_wwf_def]
       \\ pairarg_tac \\ fs []
       \\ pairarg_tac \\ fs []
       \\ pairarg_tac \\ fs []
       \\ rw [cexp_wf_def])
   >~[‘Raise’]
-  >- (fs [give_names_def, cexp_wf_def]
+  >- (fs [give_names_def, cexp_wwf_def]
       \\ pairarg_tac \\ fs []
       \\ rw [cexp_wf_def])
   >~[‘Letrec’]
-  >- (fs [give_names_def, cexp_wf_def]
+  >- (fs [give_names_def, cexp_wwf_def]
       \\ pairarg_tac \\ fs []
       \\ rw [cexp_wf_def]
       >- (gs [EVERY_EL, EL_MAP, EL_MAP2, MEM_EL, PULL_EXISTS]
@@ -254,7 +254,7 @@ Proof
       \\ pairarg_tac \\ fs []
       \\ pairarg_tac \\ fs [])
   >~[‘Case _ rows d’]
-  >- (fs [give_names_def, cexp_wf_def]
+  >- (fs [give_names_def, cexp_wwf_def]
       \\ Cases_on ‘d’ \\ fs []
       \\ rw [cexp_wf_def]
       >- (Cases_on ‘rows’ \\ fs [])
@@ -392,13 +392,13 @@ Proof
 QED
 
 Theorem give_all_names_cexp_wf:
-  cexp_wf x ⇒
+  cexp_wwf x ⇒
   cexp_wf (give_all_names x) ∧
   cns_arities (give_all_names x) = cns_arities x
 Proof
   fs [give_all_names_def]
   \\ Cases_on ‘give_names x’
-  \\ drule_then assume_tac give_names_cexp_wf
+  \\ drule_then assume_tac give_names_cexp_wwf
   \\ drule_then assume_tac give_names_cns_arities
   \\ fs []
 QED
